feat: Structure refactoring and some faster proofs

Valaig/Aig/Basic.lean
@@ -1,364 +1,54 @@
 import Std.Sat.AIG.Basic
 import Std.Sat.AIG.CachedGates
-import Valaig.Aig.StdSatLemmas
-
-namespace Valaig
-namespace Aig
-
-structure Var where
-  ofIdx ::
-    idx : Nat
-deriving Hashable, DecidableEq, Repr, Inhabited, Ord, BEq, ReflBEq, LawfulBEq
-
-instance : LE Var := leOfOrd
-instance : LT Var := ltOfOrd
-
-instance : EquivBEq Var where
-  symm := by simp [BEq.beq, instBEqVar.beq]; omega
-  trans := by simp [BEq.beq, instBEqVar.beq]; omega
-
-instance : LawfulHashable Var where
-  hash_eq := by
-    simp [BEq.beq, instBEqVar.beq, Hashable.hash, instHashableVar.hash]
-    grind only
-
-namespace Var
-
-@[inline]
-def constant : Var :=
-  .ofIdx 0
-
-@[inline]
-def offset (v : Var) (n : Nat) : Var :=
-  .ofIdx <| (v.idx + n)
-
-@[inline]
-def next (v : Var) : Var :=
-  v.offset 1
-
-@[inline, simp, grind .]
-def ofRef {α} [DecidableEq α] [Hashable α] {aig : Std.Sat.AIG α} (ref : aig.Ref) : Var :=
-  .ofIdx ref.gate
-
-end Var
-
-structure Lit where
-  ofIdx ::
-    idx : Nat
-deriving Hashable, DecidableEq, Repr, Inhabited, BEq
-
-namespace Lit
-
-@[inline]
-def mk (v : Var) (invert : Bool := false) : Lit :=
-  .ofIdx <| v.idx * 2 ||| invert.toNat
-
-@[inline]
-def var (l : Lit) : Var :=
-  .ofIdx <| l.idx / 2
-
-@[inline]
-def invert (l : Lit) : Lit :=
-  .ofIdx <| l.idx ^^^ 1
-
-@[inline]
-def inverted (l : Lit) : Bool :=
-  (l.idx &&& 1) ≠ 0
-
-@[inline]
-def defines (l : Lit) : Option Var :=
-  if !l.inverted then some l.var else none
-
-@[inline]
-def isConstant (l : Lit) : Bool :=
-  l.var = .constant
-
-@[inline]
-def isFalse (l : Lit) : Bool :=
-  l.isConstant ∧ !l.inverted
-
-@[inline]
-def isTrue (l : Lit) : Bool :=
-  l.isConstant ∧ l.inverted
-
-@[inline]
-def constant (value : Bool) : Lit :=
-  mk .constant value
-
-@[inline]
-def false : Lit :=
-  constant .false
-
-@[inline]
-def true : Lit :=
-  constant .true
-
-@[inline]
-def ofFanin (fi : Std.Sat.AIG.Fanin) : Lit :=
-  .mk (.ofIdx fi.gate) fi.invert
-
-@[simp]
-theorem mk_var (var : Var) {invert : Bool} :
-    (Lit.mk var invert).var = var := by
-  simp [mk, Lit.var, Nat.or_div_two]
-  have : invert.toNat / 2 = 0 := by
-    have := Bool.toNat_le invert
-    omega
-  simp [this]
-
-@[simp]
-theorem mk_inverted {v : Var} (invert : Bool) :
-    (Lit.mk v invert).inverted = invert := by
-  simp [mk, inverted]
-  decide +revert
-
-section
-variable {α} [DecidableEq α] [Hashable α] {aig : Std.Sat.AIG α}
-
-@[inline]
-def ofRef (ref : aig.Ref) : Lit :=
-  .mk (.ofRef ref) ref.invert
-
-@[inline]
-def toRef (lit : Lit) (h : lit.var.idx < aig.decls.size) : aig.Ref :=
-  .mk lit.var.idx lit.inverted h
-
-@[simp]
-theorem ofRef_var_idx_eq_gate (ref : aig.Ref) :
-    (ofRef ref |>.var.idx) = ref.gate := by
-  simp [ofRef]
-
-end
-
-end Lit
-
-namespace Var
-
-@[inline]
-abbrev toLit (v : Var) (invert : Bool := false) : Lit :=
-  Lit.mk v invert
-
-attribute [coe] toLit
-instance : Coe Var Lit where
-  coe := toLit
-
-end Var
-
-/--
-The metadata of an input in the Aig
--/
-structure Input where
-  var : Var
-  symbol : String := ""
-deriving Hashable, DecidableEq, Repr, Inhabited
-
-namespace Input
-
-@[inline]
-abbrev idx (input : Input) : Nat :=
-  input.var.idx
-
-@[inline]
-abbrev lit (input : Input) : Lit :=
-  input.var
-
-attribute [coe] Input.var
-instance : Coe Input Var where
-  coe := Input.var
-
-end Input
-
-/--
-The metadata of a latch in the Aig
--/
-structure Latch where
-  var : Var
-  next : Option Lit
-  reset : Option Lit := none
-  symbol : String := ""
-deriving Hashable, DecidableEq, Repr, Inhabited
-
-namespace Latch
-
-@[inline]
-abbrev idx (latch : Latch) : Nat :=
-  latch.var.idx
-
-@[inline]
-abbrev lit (latch : Latch) : Lit :=
-  latch.var
-
-attribute [coe] Latch.var
-instance : Coe Latch Var where
-  coe := Latch.var
-
-end Latch
-
-/--
-An atom in the combinational aig is either an input or a latch, which is just
-a reference back to the index in the inputs or latches arrays
--/
-inductive Atom where
-| input (idx : Nat) : Atom
-| latch (idx : Nat) : Atom
-deriving Hashable, DecidableEq, Repr, Inhabited
-
-/--
-An output of interest in the circuit - this is also used to represent other
-nameable nodes in the Aiger format like bad and constraint nodes
--/
-structure Output where
-  lit : Lit
-  symbol : String := ""
-deriving Hashable, DecidableEq, Repr, Inhabited
-
-abbrev Inputs := Array Input
-abbrev Latches := Array Latch
-abbrev Outputs := Array Output
-
-section
-open Std.Sat AIG
-
-@[simp]
-abbrev InputsInj (inputs : Inputs) (aig : AIG Atom) : Prop :=
-  ∀ (iin : Nat) (hinbound : iin < inputs.size),
-  ∃ (hdeclbound : inputs[iin].idx  < aig.decls.size),
-    aig.decls[inputs[iin].idx] = .atom (.input iin)
-
-@[simp]
-abbrev InputsSur (inputs : Inputs) (aig : AIG Atom) : Prop :=
-  ∀ (idecl : Nat) (hdeclbound : idecl < aig.decls.size),
-  match aig.decls[idecl] with
-  | .atom (.input iin) =>
-    ∃ (hinbound: iin < inputs.size), inputs[iin].idx = idecl
-  | _ => true
-
-@[grind]
-structure InputsBij (inputs : Inputs) (aig : AIG Atom) : Prop where
-  hinjec : InputsInj inputs aig
-  hsurjec : InputsSur inputs aig
-
-attribute [simp] InputsBij.mk
-
-@[simp]
-abbrev LatchesInj (latches : Latches) (aig : AIG Atom) : Prop :=
-  ∀ (ilat : Nat) (hlatbound : ilat < latches.size),
-  ∃ (hdeclbound : latches[ilat].idx  < aig.decls.size),
-    aig.decls[latches[ilat].idx] = .atom (.latch ilat)
-
-@[simp]
-abbrev LatchesSur (latches : Latches) (aig : AIG Atom) : Prop :=
-  ∀ (idecl : Nat) (hdeclbound : idecl < aig.decls.size),
-  match aig.decls[idecl] with
-  | .atom (.latch idx) =>
-    ∃ (hlatbound: idx < latches.size), latches[idx].idx = idecl
-  | _ => true
-
-@[grind]
-structure LatchesBij (latches : Latches) (aig : AIG Atom) : Prop where
-  hinjec : LatchesInj latches aig
-  hsurjec : LatchesSur latches aig
-
-attribute [simp] LatchesBij.mk
-
-end
-
-end Aig
-
-/--
-An Aig with added sequential semantics through latches and Aiger style outputs,
-We add a number of invariants to preserve that keeps the Aig in a state where
-it is easier to reason about/manipulate and that are practical for a future
-optimized implementation.
--/
-structure Aig where
-  -- The underlying AIG
-  aig : Std.Sat.AIG Aig.Atom
-
-  -- A mapping from input indices (Atom.input idx) to their definition
-  inputs : Aig.Inputs
-
-  -- A mapping from latch indices (Atom.latch idx) to their definition
-  latches : Aig.Latches
-
-  -- A set of literals that should never be true
-  bads : Aig.Outputs
-
-  -- Only index 0 represents false
-  hfalse : ∀ (i : Nat) (h : i < aig.decls.size), aig.decls[i] = .false ↔ i = 0
-
-  -- There is a bijection between indices in the inputs array and input atoms
-  -- in the aig
-  hinputmap : Aig.InputsBij inputs aig
-
-  -- There is a bijection between indices in the latches array and latch atoms
-  -- in the aig
-  hlatchmap : Aig.LatchesBij latches aig
-
-  -- Resets are stratified. TODO: This definition doesn't work as the binary
-  -- aiger format requires latches come before gates, so you can't define
-  -- interesting reset conditions like this. Instead I think we just want a
-  -- generalized form (maybe we should also be able to switch to a mode where
-  -- this more restrictive constraint is used, it makes checking for cycles etc
-  -- way easier)
-  -- hreset : ∀ {latch}, latch ∈ latches → latch.reset.var < latch.var
-
-structure Aig.WF (aig : Aig) where
-  -- We specify that each latch must have a next state as an external
-  -- well-formedness predicate as
-  hnext : ∀ {latch}, latch ∈ aig.latches → latch.next.isSome
-
-  -- TODO: Should other predicates be here too? There are other cases when it
-  -- could be nice to be able to momentarily break invariants, in particular
-  -- hreset
-
--- Allow grind to get at the Aig invariants
-attribute [grind =] Aig.aig
-attribute [grind! .] Std.Sat.AIG.hzero
-attribute [grind! .] Std.Sat.AIG.hconst
-attribute [grind =] Aig.hfalse
-attribute [grind! .] Aig.hinputmap
-attribute [grind! .] Aig.hlatchmap
-
-namespace Aig
+import Valaig.Aig.Defs
+import Valaig.Aig.DefsLemmas
+import Valaig.Aig.RefsLemmas
+
+namespace Valaig.Aig.Raw
 
 @[inline, simp]
-abbrev size (aig : Aig) : Nat := aig.aig.decls.size
+abbrev size (aig : Raw) : Nat := aig.aig.decls.size
 
-@[inline]
-abbrev numConstants (_ : Aig) : Nat := 1
+@[inline, simp]
+abbrev numInputs (aig : Raw) : Nat := aig.inputs.size
 
-@[inline]
-abbrev numInputs (aig : Aig) : Nat := aig.inputs.size
-
-@[inline]
-abbrev numLatches (aig : Aig) : Nat := aig.latches.size
+@[inline, simp]
+abbrev numLatches (aig : Raw) : Nat := aig.latches.size
 
 -- Number of inputs and latches
+@[inline, simp, grind]
+def numAtoms (aig : Raw) : Nat := aig.numInputs + aig.numLatches
+
 @[inline]
-def numAtoms (aig : Aig) : Nat := aig.numInputs + aig.numLatches
+def maxVar (aig : Raw) : Var := .ofIdx (aig.size - 1)
+
+@[inline, simp]
+abbrev numConstants (_ : Raw) : Nat := 1
 
 -- Number of inputs, latches and constants
-@[inline]
-def numLeaves (aig : Aig) : Nat := aig.numAtoms + aig.numConstants
+@[inline, simp, grind]
+def numLeaves (aig : Raw) : Nat := aig.numAtoms + aig.numConstants
+
+@[inline, simp, grind]
+def numGates (aig : Raw) : Nat := aig.size - aig.numLeaves
+
+end Aig.Raw
 
 @[inline]
-def numGates (aig : Aig) : Nat := aig.size - aig.numLeaves
+def Var.validIn (var : Var) (aig : Aig) :=
+  var.idx < aig.size
 
-@[inline]
-abbrev numBads (aig : Aig) : Nat := aig.bads.size
-
-@[inline]
-def maxVar (aig : Aig) : Var := .ofIdx (aig.size - 1)
-
-@[inline]
-def Var.validIn (var : Var) (aig : Aig) := var.idx < aig.size
-
-@[inline]
+@[inline, simp]
 abbrev Lit.validIn (lit : Lit) (aig : Aig) := lit.var.validIn aig
 
 abbrev Var.In (aig : Aig) := { var : Var // var.validIn aig }
 abbrev Lit.In (aig : Aig) := { lit : Lit // lit.validIn aig }
+
+namespace Aig
+
+instance : GetElem Aig Var (Std.Sat.AIG.Decl Atom) (fun aig var => var.validIn aig) where
+  getElem aig var (h := by grind) :=
+    aig.aig.decls[var.idx]
 
 @[inline]
 def empty : Aig :=
@@ -366,41 +56,36 @@ def empty : Aig :=
     aig := .empty
     inputs := #[],
     latches := #[],
-    bads := #[],
     hfalse := by simp [Std.Sat.AIG.empty],
-    hinputmap := by simp [Std.Sat.AIG.empty],
-    hlatchmap := by simp [Std.Sat.AIG.empty],
+    hinputs := by simp [Std.Sat.AIG.empty],
+    hlatches := by simp [Std.Sat.AIG.empty],
   }
 
 @[inline]
-abbrev nextInputIdx (aig : Aig) : Nat :=
+def nextInputIdx (aig : Aig) : Nat :=
   aig.numInputs
 
 @[inline]
-abbrev nextLatchIdx (aig : Aig) : Nat :=
+def nextLatchIdx (aig : Aig) : Nat :=
   aig.numLatches
-
-theorem nextInputIdx_notIn_decls (aig : Aig) {i : Nat} (h : i < aig.size) :
-    aig.aig.decls[i] ≠ .atom (.input aig.nextInputIdx) := by
-  grind
-
-theorem nextLatchIdx_notIn_decls (aig : Aig) {i : Nat} (h : i < aig.size) :
-    aig.aig.decls[i] ≠ .atom (.latch aig.nextLatchIdx) := by
-  grind
 
 @[inline]
 def addInput (aig : Aig) (symbol : String := "") : Aig × Input :=
   -- We don't need to use mkAtomCached as nextInputIdx_notIn_decls guarantees
   -- it would be a miss
-  let res := aig.aig.mkAtom <| .input aig.nextInputIdx
+  let atom := (.input aig.nextInputIdx)
+  let res := aig.aig.mkAtom atom
   let input := { var := .ofRef res.ref, symbol }
 
   let aig := { aig with
     aig := res.aig,
     inputs := aig.inputs.push input,
-    hfalse := by grind,
-    hinputmap := by grind,
-    hlatchmap := by grind,
+    hfalse := by apply hfalse_decls_push ?_ (by apply mkAtom_eq_decls_push) <;> grind only [hfalse],
+    hinputs := by
+      apply AtomsBij_push_push (by apply mkAtom_eq_decls_push) (by trivial) (hbijec := aig.hinputs)
+      · grind only [mkAtom_ref_eq_decls_size, Var.ofRef_idx]
+      · grind only [nextInputIdx]
+    hlatches := by apply AtomsBij_unchanged_push (by apply mkAtom_eq_decls_push) <;> grind only [hlatches],
   }
   (aig, input)
 
@@ -419,9 +104,12 @@ def addLatch (aig : Aig) (next : Lit) (reset : Option Lit := none) (symbol : Str
   let aig := { aig with
     aig := res.aig,
     latches := aig.latches.push latch,
-    hfalse := by grind,
-    hinputmap := by grind,
-    hlatchmap := by grind,
+    hfalse := by apply hfalse_decls_push ?_ (by apply mkAtom_eq_decls_push) <;> grind only [hfalse],
+    hinputs := by apply AtomsBij_unchanged_push (by apply mkAtom_eq_decls_push) <;> grind only [hinputs],
+    hlatches := by
+      apply AtomsBij_push_push (by apply mkAtom_eq_decls_push) (by trivial) (hbijec := aig.hlatches)
+      · grind only [mkAtom_ref_eq_decls_size, Var.ofRef_idx]
+      · grind only [nextLatchIdx]
   }
   (aig, latch)
 
@@ -440,9 +128,12 @@ def addLatch' (aig : Aig) (reset : Option Lit := none) (symbol : String := "") :
   let aig := { aig with
     aig := res.aig,
     latches := aig.latches.push latch,
-    hfalse := by grind,
-    hinputmap := by grind,
-    hlatchmap := by grind,
+    hfalse := by apply hfalse_decls_push ?_ (by apply mkAtom_eq_decls_push) <;> grind only [hfalse],
+    hinputs := by apply AtomsBij_unchanged_push (by apply mkAtom_eq_decls_push) <;> grind only [hinputs],
+    hlatches := by
+      apply AtomsBij_push_push (by apply mkAtom_eq_decls_push) (by trivial) (hbijec := aig.hlatches)
+      · grind only [mkAtom_ref_eq_decls_size, Var.ofRef_idx]
+      · grind only [nextLatchIdx]
   }
   (aig, latch)
 
@@ -452,17 +143,24 @@ def addGate (aig : Aig) (rhs0 rhs1 : Lit)
     Aig × Lit :=
   let res := aig.aig.mkAndCached ⟨rhs0.toRef h0, rhs1.toRef h1⟩
 
+
   let aig := { aig with
     aig := res.aig,
     hfalse := by
-      intro i
-      by_cases i < aig.size
-      · grind
-      · -- For some reason if I remove this grind hits an error
-        have : i ≠ 0 := by grind only [Std.Sat.AIG.hzero]
-        grind,
-    hinputmap := by grind
-    hlatchmap := by grind
+      apply hfalse_decls_append aig.hfalse
+      · grind only [Std.Sat.AIG.mkAndCached_decl_eq]
+      · grind only [mkAndCached_matches_gate]
+      · apply Std.Sat.AIG.mkAndCached_le_size,
+    hinputs := by
+      apply AtomsBij_unchanged_append aig.hinputs
+      · apply Std.Sat.AIG.mkAndCached_le_size
+      · grind only [Std.Sat.AIG.mkAndCached_decl_eq]
+      · grind only [mkAndCached_matches_gate],
+    hlatches := by
+      apply AtomsBij_unchanged_append aig.hlatches
+      · apply Std.Sat.AIG.mkAndCached_le_size
+      · grind only [Std.Sat.AIG.mkAndCached_decl_eq]
+      · grind only [mkAndCached_matches_gate],
   }
   (aig, Lit.ofRef res.ref)
 
@@ -475,20 +173,22 @@ def addGateUncached (aig : Aig) (rhs0 rhs1 : Lit)
   let aig := { aig with
     aig := res.aig,
     hfalse := by
-      intro i
-      by_cases i < aig.size
-      · grind
-      · -- For some reason if I remove this grind hits an error
-        have : i ≠ 0 := by grind only [Std.Sat.AIG.hzero]
-        grind,
-    hinputmap := by grind
-    hlatchmap := by grind
+      apply hfalse_decls_append aig.hfalse
+      · grind only [Std.Sat.AIG.mkGate_decl_eq]
+      · grind only [mkGate_matches_gate]
+      · apply Std.Sat.AIG.mkGate_le_size,
+    hinputs := by
+      apply AtomsBij_unchanged_append aig.hinputs
+      · apply Std.Sat.AIG.mkGate_le_size
+      · grind only [Std.Sat.AIG.mkGate_decl_eq]
+      · grind only [mkGate_matches_gate],
+    hlatches := by
+      apply AtomsBij_unchanged_append aig.hlatches
+      · apply Std.Sat.AIG.mkGate_le_size
+      · grind only [Std.Sat.AIG.mkGate_decl_eq]
+      · grind only [mkGate_matches_gate]
   }
   (aig, Lit.ofRef res.ref)
-
-@[inline]
-def addBad (aig : Aig) (lit : Lit) (symbol : String := "") (_h : lit.validIn aig := by grind) : Aig :=
-  { aig with bads := aig.bads.push { lit, symbol } }
 
 @[unbox, grind]
 structure FinaliseLatchesState (aig : Aig) where
@@ -501,7 +201,7 @@ structure FinaliseLatchesState (aig : Aig) where
 @[inline]
 def finaliseLatches (aig : Aig) (nextState : (latch : Latch) -> latch ∈ aig.latches -> Lit.In aig) : Aig :=
   have s := updateLatches
-  { aig with latches := s.latches, hlatchmap := by grind}
+  { aig with latches := s.latches, hlatches := by grind}
 
 where
   updateLatches (s : FinaliseLatchesState aig := {}) : FinaliseLatchesState aig :=
@@ -509,7 +209,7 @@ where
       s
     else
       match s.latches[s.idx].next with
-      | some _ => updateLatches { s with idx := s.idx + 1, habove := by grind }
+      | some _ => updateLatches { s with idx := s.idx + 1, habove := by grind only }
       | none =>
         let next := nextState s.latches[s.idx] (by grind)
         let latches := s.latches.modify s.idx fun latch => { latch with next }
@@ -518,7 +218,7 @@ where
           idx := s.idx + 1,
           hsize := by grind,
           habove := by grind,
-          hvar := by grind
+          hvar := by grind,
         }
         updateLatches s
 
