Valaig.lean
@@ -1,2 +1,3 @@
 import Valaig.Aig
+import Valaig.Aiger
 import Valaig.External
