Valaig/Aig.lean
@@ -1,4 +1,6 @@
+import Valaig.Aig.Refs
+import Valaig.Aig.RefsLemmas
+import Valaig.Aig.Defs
 import Valaig.Aig.Basic
 import Valaig.Aig.Lemmas
-import Valaig.Aig.Aiger
-import Valaig.Aig.Result
+import Valaig.Aig.FromStd
