Valaig/Aig/Aiger.lean
@@ -1,2 +1,0 @@
-import Valaig.Aig.Aiger.Parser
-import Valaig.Aig.Aiger.Writer
