Valaig/Aig/Defs.lean
@@ -1,0 +1,170 @@
+import Valaig.Aig.Refs
+
+namespace Valaig.Aig
+
+-- We define VarDef and WithSymbol for the two fields that both Inputs/Latches
+-- have separately so they are transparently inlined into Inputs/Latches
+structure VarDef where
+  var : Var
+deriving Hashable, DecidableEq, Repr, Inhabited, BEq
+
+namespace VarDef
+
+@[inline, simp]
+abbrev idx (self : VarDef) : Nat :=
+  self.var.idx
+
+@[inline, simp]
+abbrev lit (self : VarDef) : Lit :=
+  self.var
+
+end VarDef
+
+structure WithSymbol where
+  symbol : String := ""
+deriving Hashable, DecidableEq, Repr, Inhabited, BEq
+
+/--
+The metadata of an input in the Aig
+-/
+structure Input extends VarDef, WithSymbol
+deriving Hashable, DecidableEq, Repr, Inhabited
+
+instance : Coe Input Var where
+  coe := (·.var)
+
+/--
+The metadata of a latch in the Aig
+-/
+structure Latch extends VarDef, WithSymbol where
+  next : Option Lit
+  reset : Option Lit := none
+deriving Hashable, DecidableEq, Repr, Inhabited
+
+instance : Coe Latch Var where
+  coe := (·.var)
+
+/--
+An atom in the combinational aig is either an input or a latch, which is just
+a reference back to the index in the inputs or latches arrays
+-/
+inductive Atom where
+| input (idx : Nat) : Atom
+| latch (idx : Nat) : Atom
+deriving Hashable, DecidableEq, Repr, Inhabited
+
+/--
+An output of interest in the circuit - this is also used to represent other
+nameable nodes in the Aiger format like bad and constraint nodes
+-/
+structure Output extends WithSymbol where
+  lit : Lit
+deriving Hashable, DecidableEq, Repr, Inhabited
+
+abbrev Inputs := Array Input
+abbrev Latches := Array Latch
+abbrev Outputs := Array Output
+
+/--
+A raw sequential Aig without any well-formedness invariants. This lets
+us define the invariants directly on this, rather than on its fields indirectly
+-/
+structure Raw where
+  -- The underlying AIG
+  aig : Std.Sat.AIG Aig.Atom
+
+  -- A mapping from input indices (Atom.input idx) to their definition
+  inputs : Inputs
+
+  -- A mapping from latch indices (Atom.latch idx) to their definition
+  latches : Latches
+
+section
+open Std.Sat AIG
+variable {α : Type} (arr : Array α) (idx : α -> Nat)
+variable (decls: Array (Decl Atom)) (mkAtom : Nat -> Atom)
+
+@[simp]
+abbrev AtomsInj : Prop :=
+  ∀ {iarr : Nat} (harrbound : iarr < arr.size),
+  ∃ (hdeclbound : idx arr[iarr] < decls.size),
+     decls[idx arr[iarr]] = .atom (mkAtom iarr)
+
+@[simp]
+abbrev AtomsSur : Prop :=
+  ∀ {idecl : Nat} (hdeclbound : idecl < decls.size),
+  ∀ {iarr : Nat} (hdecl : decls[idecl] = .atom (mkAtom iarr)),
+  ∃ (harrbound: iarr < arr.size),
+    idx arr[iarr] = idecl
+
+@[grind]
+structure AtomsBij : Prop where
+  hinjec : AtomsInj arr idx decls mkAtom
+  hsurjec : AtomsSur arr idx decls mkAtom
+
+attribute [simp] AtomsBij.mk
+
+end
+
+namespace Raw
+
+@[simp]
+abbrev InputsBij (aig : Raw) :=
+  AtomsBij aig.inputs (·.idx) aig.aig.decls Atom.input
+
+@[simp]
+abbrev LatchesBij (aig : Raw) :=
+  AtomsBij aig.latches (·.idx) aig.aig.decls Atom.latch
+
+@[simp]
+abbrev SingleFalse (aig : Raw) :=
+  ∀ {i : Nat} (h : i < aig.aig.decls.size), aig.aig.decls[i] = .false ↔ i = 0
+
+@[simp]
+abbrev NextStateDefined (aig : Raw) :=
+  ∀ {latch} (_ : latch ∈ aig.latches), latch.next.isSome
+
+end Aig.Raw
+
+/--
+An Aig with added sequential semantics through latches.
+We add a number of invariants to preserve that keeps the Aig in a state where
+it is easier to reason about/manipulate and that are practical for a future
+optimized implementation.
+-/
+structure Aig extends Aig.Raw where
+  -- Only index 0 represents false
+  hfalse : toRaw.SingleFalse
+
+  -- There is a bijection between indices in the inputs array and input atoms
+  -- in the aig
+  hinputs : toRaw.InputsBij
+
+  -- There is a bijection between indices in the latches array and latch atoms
+  -- in the aig
+  hlatches : toRaw.LatchesBij
+
+attribute [grind] Aig.Raw.aig
+attribute [grind! .] Std.Sat.AIG.hzero
+attribute [grind! .] Std.Sat.AIG.hconst
+attribute [grind! .] Aig.hfalse
+attribute [grind! .] Aig.hinputs
+attribute [grind! .] Aig.hlatches
+
+instance : Coe Aig Aig.Raw where
+  coe := (·.toRaw)
+
+structure Aig.WF (aig : Aig) where
+  -- We specify that each latch must have a next state as an external
+  -- well-formedness predicate as
+  hnext : aig.toRaw.NextStateDefined
+
+  -- Resets are stratified. TODO: This definition doesn't work as the binary
+  -- aiger format requires latches come before gates, so you can't define
+  -- interesting reset conditions like this. Instead I think we just want a
+  -- generalized form (maybe we should also be able to switch to a mode where
+  -- this more restrictive constraint is used, it makes checking for cycles etc
+  -- way easier)
+  -- hreset : ∀ {latch}, latch ∈ latches → latch.reset.var < latch.var
+
+end Valaig
