Valaig/Aig/DefsLemmas.lean
@@ -1,0 +1,135 @@
+import Valaig.Aig.Defs
+import Valaig.Aig.StdSatLemmas
+
+namespace Valaig.Aig
+
+-- -- When proving a property motive that quantifies over all indices of a pushed
+-- -- array, split it into two cases for the indices in the old array and the index
+-- -- of the new array. This is designed to be used as apply push_forall_cases h.
+-- -- To allow the motive to pattern match, it takes the same form each time but
+-- -- we add extra predicates that simp can use to rewrite the motive for each case
+-- theorem push_forall_cases {α : Type} {xs : Array α} {x : α}
+--     {i : Nat} (hi : i < (xs.push x).size)
+--     {motive : (i : Nat) -> i < (xs.push x).size -> Prop}
+--     (hlt :
+--       ∀ (hi : i < xs.size)
+--         {hp : (xs.push x)[i]'(by grind only [Array.size_push]) = xs[i]},
+--           motive i (by grind only [Array.size_push]))
+--     (heq :
+--       ∀ {h : (xs.push x)[xs.size] = x},
+--         motive xs.size (by grind only [Array.size_push])) :
+--     motive i hi := by
+--   grind only [Array.size_push, Array.getElem_push]
+
+section
+variable {aig aig' : Raw}
+
+theorem hfalse_decls_push {atom}
+    (hfalse : aig.SingleFalse)
+    (heq : aig'.aig.decls = aig.aig.decls.push atom)
+    (hatom : atom ≠ .false) :
+    aig'.SingleFalse := by
+  grind only [Std.Sat.AIG.hzero, Array.size_push, Array.getElem_push]
+
+theorem hfalse_decls_append
+    (hfalse : aig.SingleFalse)
+    (hsize : aig'.aig.decls.size ≥ aig.aig.decls.size)
+    (hlt :
+      ∀ {i} (hi : i < aig.aig.decls.size),
+        aig'.aig.decls[i] = aig.aig.decls[i])
+    (happend :
+      ∀ {i} (_hlow : i ≥ aig.aig.decls.size) (hhigh : i < aig'.aig.decls.size),
+        aig'.aig.decls[i] ≠ .false) :
+    aig'.SingleFalse := by
+  grind only [Std.Sat.AIG.hzero]
+
+end
+
+section
+
+variable {arr arr' : Array α} {idx : α -> Nat}
+variable {decls decls': Array (Std.Sat.AIG.Decl Atom)}
+variable {mkAtom : Nat -> Atom}
+
+section
+
+variable {atom : Std.Sat.AIG.Decl Atom}
+variable (heq : decls' = decls.push atom)
+variable (hatom : ∀ {idx}, atom ≠ .atom (mkAtom idx))
+include heq hatom
+
+omit hatom in
+theorem AtomsInj_unchanged_push (hinjec : AtomsInj arr idx decls mkAtom) :
+    AtomsInj arr idx decls' mkAtom := by
+  grind only [Array.size_push, Array.getElem_push]
+
+theorem AtomsSur_unchanged_push (hsurjec : AtomsSur arr idx decls mkAtom) :
+    AtomsSur arr idx decls' mkAtom := by
+  grind only [Array.size_push, Array.getElem_push]
+
+theorem AtomsBij_unchanged_push (hbijec : AtomsBij arr idx decls mkAtom) :
+    AtomsBij arr idx decls' mkAtom := by
+  constructor
+  · exact AtomsInj_unchanged_push heq hbijec.hinjec
+  · exact AtomsSur_unchanged_push heq hatom hbijec.hsurjec
+
+end
+
+section
+
+variable {item : α}
+variable {atom : Std.Sat.AIG.Decl Atom}
+variable (hdecls : decls' = decls.push atom)
+variable (harr : arr' = arr.push item)
+variable (hidx : idx item = decls.size)
+variable (hatom : atom = .atom (mkAtom arr.size))
+variable (hMkAtomInj : ∀ {i j}, mkAtom i = mkAtom j ↔ i = j := by simp_all)
+include hdecls harr hidx hatom
+
+theorem AtomsInj_push_push (hinjec : AtomsInj arr idx decls mkAtom) :
+    AtomsInj arr' idx decls' mkAtom := by
+  grind only [Array.size_push, Array.getElem_push]
+
+include hMkAtomInj
+theorem AtomsSur_push_push (hsurjec : AtomsSur arr idx decls mkAtom) :
+    AtomsSur arr' idx decls' mkAtom := by
+  grind only [Array.size_push, Array.getElem_push]
+
+include hMkAtomInj
+theorem AtomsBij_push_push (hbijec : AtomsBij arr idx decls mkAtom) :
+    AtomsBij arr' idx decls' mkAtom := by
+  constructor
+  · exact AtomsInj_push_push hdecls harr hidx hatom (hinjec := hbijec.hinjec)
+  · exact AtomsSur_push_push hdecls harr hidx hatom (hsurjec := hbijec.hsurjec)
+
+end
+
+section
+
+variable {hsize : decls'.size ≥ decls.size}
+variable {hlt : ∀ {i} (hi : i < decls.size), decls'[i] = decls[i]}
+variable
+  {happend :
+    ∀ {i} (_hlow : i ≥ decls.size) (hhigh : i < decls'.size),
+    ∀ {idx}, decls'[i] ≠ .atom (mkAtom idx)}
+include hsize hlt happend
+
+theorem AtomsInj_unchanged_append (hinjec : AtomsInj arr idx decls mkAtom) :
+    AtomsInj arr idx decls' mkAtom := by
+  grind only
+
+theorem AtomsSur_unchanged_append (hsurjec : AtomsSur arr idx decls mkAtom) :
+    AtomsSur arr idx decls' mkAtom := by
+  grind only
+
+theorem AtomsBij_unchanged_append (hbijec : AtomsBij arr idx decls mkAtom) :
+    AtomsBij arr idx decls' mkAtom := by
+  constructor
+  · exact AtomsInj_unchanged_append hbijec.hinjec (hsize := hsize) (hlt := hlt) (happend := happend)
+  · exact AtomsSur_unchanged_append hbijec.hsurjec (hsize := hsize) (hlt := hlt) (happend := happend)
+
+end
+
+end
+
+end Valaig.Aig
