Valaig/Aig/Refs.lean
@@ -1,0 +1,136 @@
+import Std.Sat.AIG.Basic
+
+namespace Valaig
+
+/--
+Variable: a reference to a node in an Aig based on its index
+-/
+structure Var where
+  ofIdx ::
+    idx : Nat
+deriving Hashable, DecidableEq, Repr, Inhabited, Ord, BEq, ReflBEq, LawfulBEq
+
+instance : LE Var := leOfOrd
+instance : LT Var := ltOfOrd
+
+instance : EquivBEq Var where
+  symm := by simp [BEq.beq, instBEqVar.beq]; omega
+  trans := by simp [BEq.beq, instBEqVar.beq]; omega
+
+instance : LawfulHashable Var where
+  hash_eq := by
+    simp only [BEq.beq, instBEqVar.beq, Hashable.hash, instHashableVar.hash, decide_eq_true_eq]
+    intros
+    congr
+
+namespace Var
+
+@[inline]
+def constant : Var :=
+  .ofIdx 0
+
+@[inline]
+def offset (v : Var) (n : Nat) : Var :=
+  .ofIdx <| (v.idx + n)
+
+@[inline]
+def next (v : Var) : Var :=
+  v.offset 1
+
+@[inline]
+def ofRef {α} [DecidableEq α] [Hashable α] {aig : Std.Sat.AIG α} (ref : aig.Ref) : Var :=
+  .ofIdx ref.gate
+
+end Var
+
+/--
+Literal: a reference to a variable in an Aig and an inversion
+-/
+structure Lit where
+  ofIdx ::
+    idx : Nat
+deriving Hashable, DecidableEq, Repr, Inhabited, BEq
+
+namespace Lit
+
+@[inline]
+def mk (v : Var) (invert : Bool := false) : Lit :=
+  .ofIdx <| v.idx * 2 ||| invert.toNat
+
+@[inline]
+def var (l : Lit) : Var :=
+  .ofIdx <| l.idx / 2
+
+@[inline]
+def inverted (l : Lit) : Prop :=
+  (l.idx &&& 1) ≠ 0
+deriving Decidable
+
+@[inline]
+def constant (value : Bool) : Lit :=
+  mk .constant value
+
+@[inline]
+def false : Lit :=
+  constant .false
+
+@[inline]
+def true : Lit :=
+  constant .true
+
+@[inline]
+def isConstant (l : Lit) : Prop :=
+  l.var = .constant
+deriving Decidable
+
+@[inline]
+def isFalse (l : Lit) : Prop :=
+  l = false
+deriving Decidable
+
+@[inline]
+def isTrue (l : Lit) : Prop :=
+  l = true
+deriving Decidable
+
+@[inline]
+def invert (l : Lit) : Lit :=
+  .ofIdx <| l.idx ^^^ 1
+
+-- Clear inverted
+@[inline]
+def strip (l : Lit) : Lit :=
+  .ofIdx <| l.idx ^^^ (l.idx &&& 1)
+
+@[inline]
+def ofFanin (fi : Std.Sat.AIG.Fanin) : Lit :=
+  mk (.ofIdx fi.gate) fi.invert
+
+section
+variable {α} [DecidableEq α] [Hashable α] {aig : Std.Sat.AIG α}
+
+@[inline]
+def ofRef (ref : aig.Ref) : Lit :=
+  mk (.ofRef ref) ref.invert
+
+@[inline]
+def toRef (lit : Lit) (h : lit.var.idx < aig.decls.size) : aig.Ref :=
+  .mk lit.var.idx lit.inverted h
+
+end
+
+end Lit
+
+namespace Var
+
+@[inline, simp]
+abbrev toLit (v : Var) (invert : Bool := false) : Lit :=
+  .mk v invert
+
+attribute [coe] toLit
+instance : Coe Var Lit where
+  coe := toLit
+
+end Var
+
+end Valaig
