Valaig/Aig/RefsLemmas.lean
@@ -1,0 +1,134 @@
+import Valaig.Aig.Refs
+
+namespace Valaig
+
+namespace Var
+
+variable {α} [DecidableEq α] [Hashable α] {aig : Std.Sat.AIG α}
+@[simp, grind =]
+theorem ofRef_idx (ref : aig.Ref) :
+    (ofRef ref).idx = ref.gate := by
+  simp only [ofRef]
+
+end Var
+
+namespace Lit
+variable {lit : Lit} {invert : Bool}
+
+-- These simp/grind rules are set up to normalize Lit terms to the mk
+-- constructor
+
+@[simp, grind =]
+theorem mk_var (var : Var) :
+    (Lit.mk var invert).var = var := by
+  have : invert.toNat / 2 = 0 := by
+    have := Bool.toNat_le invert
+    omega
+  rw [Lit.var, mk, Nat.or_div_two, this, Nat.or_zero, Nat.mul_div_cancel]
+  omega
+
+@[simp, grind =]
+theorem mk_inverted (var : Var) :
+    (Lit.mk var invert).inverted ↔ invert := by
+  simp [mk, inverted]
+  decide +revert
+
+theorem ext_idx (lit lit' : Lit) :
+    lit = lit' ↔ lit.idx = lit'.idx := by
+  grind only [Lit]
+
+@[grind! .]
+theorem mk_self_eq_self :
+    Lit.mk lit.var lit.inverted = lit := by
+  by_cases h : lit.inverted
+  · simp_all [mk, var, inverted, ext_idx]
+    have {a b : Nat} : a = b ↔ (a % 2) = (b % 2) ∧ (a / 2) = (b / 2) := by omega
+    rw [this]
+    simp [h, Nat.or_div_two]
+  · simp_all [mk, var, inverted, Nat.div_mul_self_eq_mod_sub_self]
+
+theorem ext {lit lit' : Lit} :
+    lit = lit' ↔ (lit.var = lit'.var ∧ lit.inverted = lit'.inverted) := by
+  grind
+
+@[simp, grind =]
+theorem mk_ext {var var' : Var} {invert invert' : Bool} :
+    (mk var invert = mk var' invert') ↔ (var = var' ∧ invert = invert') := by
+  simp [ext]
+
+@[simp, grind =]
+theorem constant_def :
+    constant invert = mk .constant invert := by
+  rw [constant]
+
+@[simp, grind =]
+theorem false_def :
+    false = constant .false := by
+  rw [false]
+
+@[simp, grind =]
+theorem true_def :
+    true = constant .true := by
+  rw [true]
+
+@[simp, grind =]
+theorem isConstant_def :
+    lit.isConstant ↔ lit.var = .constant := by
+  rw [isConstant]
+
+@[simp, grind =]
+theorem isFalse_def :
+    lit.isFalse ↔ lit = false := by
+  rw [isFalse]
+
+@[simp, grind =]
+theorem isTrue_def :
+    lit.isTrue ↔ lit = true := by
+  rw [isTrue]
+
+theorem isConstant_iff :
+    lit.isConstant ↔ lit.isFalse ∨ lit.isTrue := by
+  grind
+
+@[simp, grind =]
+theorem invert_def :
+    lit.invert = mk lit.var ¬lit.inverted := by
+  rw [Lit.ext] <;> simp
+  constructor
+  · simp [invert, var, Nat.xor_div_two]
+  · simp [invert, inverted]
+
+@[simp, grind =]
+theorem strip_def :
+    lit.strip = mk lit.var .false := by
+  rw [strip, Lit.ext] <;> simp
+  constructor
+  · simp [var, Nat.xor_div_two]
+  · simp [inverted]
+
+theorem ofFanin_def (fi : Std.Sat.AIG.Fanin) :
+    ofFanin fi = mk (.ofIdx fi.gate) fi.invert := by
+  rw [ofFanin]
+
+section
+variable {α} [DecidableEq α] [Hashable α] {aig : Std.Sat.AIG α}
+
+@[simp, grind =]
+theorem ofRef_def (ref : aig.Ref) :
+    ofRef ref = mk (.ofRef ref) ref.invert := by
+  rw [ofRef]
+
+@[simp, grind =]
+theorem toRef_gate {h : lit.var.idx < aig.decls.size} :
+    (toRef lit h).gate = lit.var.idx := by
+  rw [toRef]
+
+@[simp, grind =]
+theorem toRef_invert {h : lit.var.idx < aig.decls.size} :
+    (toRef lit h).invert = lit.inverted := by
+  simp only [toRef, decide_eq_true_eq]
+
+end
+
+end Lit
+end Valaig
