Valaig/Aig/StdSatLemmas.lean
@@ -13,54 +13,63 @@ variable {α : Type} [Hashable α] [DecidableEq α]
 /--
 `AIG.mkAtom` only appends a single atom to the underlying AIG.
 -/
-@[simp, grind! .]
 theorem mkAtom_eq_decls_push (aig : AIG α) (var : α) :
     (aig.mkAtom var).aig.decls = aig.decls.push (.atom var) := by
-  simp [mkAtom]
+  simp only [mkAtom]
+
+/--
+`AIG.mkAtom` increments size by one.
+-/
+theorem mkAtom_size (aig : AIG α) (var : α) :
+    (aig.mkAtom var).aig.decls.size = aig.decls.size + 1 := by
+  simp only [mkAtom_eq_decls_push, Array.size_push]
 
 /--
 `AIG.mkAtom` returns a reference to the next element in the underlying AIG
 -/
-@[simp, grind! .]
 theorem mkAtom_ref_eq_decls_size (aig : AIG α) (var : α) :
     (aig.mkAtom var).ref.gate = aig.decls.size := by
-  simp [mkAtom]
+  simp only [mkAtom]
 
 /--
 - `AIG.mkGate` only potentially appends gates, not atoms/constants
 -/
-@[simp, grind! .]
-theorem mkGate_matches_gate (idx : Nat) (aig : AIG α) (input : aig.BinaryInput)
+theorem mkGate_matches_gate (aig : AIG α) {input : aig.BinaryInput} {idx : Nat}
     {hlow : idx ≥ aig.decls.size} {hhigh : idx < (aig.mkGate input).aig.decls.size} :
-    (aig.mkGate input).aig.decls[idx] matches .gate _ _ := by
-  grind [mkGate]
+    ∃ (lhs rhs : Fanin), (aig.mkGate input).aig.decls[idx] = .gate lhs rhs := by
+  generalize hres : (aig.mkGate input).aig.decls = res at *
+  unfold mkGate at hres
+  have heq : idx = aig.decls.size := by
+    rw [←hres, Array.size_push] at hhigh
+    exact Nat.eq_of_le_of_lt_succ hlow hhigh
+  simp [←hres, heq]
 
-attribute [simp, grind! .] mkGate_decl_eq
-attribute [simp, grind! .] mkGate_le_size
+theorem mkGateCached.go_matches_gate (aig : AIG α) {input : aig.BinaryInput} {idx : Nat}
+    {hlow : idx ≥ aig.decls.size} {hhigh : idx < (mkGateCached.go aig input).aig.decls.size} :
+    ∃ (lhs rhs : Fanin), (mkGateCached.go aig input).aig.decls[idx] = .gate lhs rhs := by
+  generalize hres : (mkGateCached.go aig input).aig.decls = res at *
+  have : aig.decls ≠ res := by cutsat
+  dsimp only [mkGateCached, mkGateCached.go] at hres
+  split at hres
+  · trivial
+  · split at hres <;> try trivial
+    · grind only [Array.getElem_push]
 
 /--
 - `AIG.mkGateCached` only potentially appends gates, not atoms/constants
 -/
-@[simp, grind! .]
-theorem mkGateCached_matches_gate (idx : Nat) (aig : AIG α) (input : aig.BinaryInput)
+theorem mkGateCached_matches_gate (aig : AIG α) {input : aig.BinaryInput} {idx : Nat}
     {hlow : idx ≥ aig.decls.size} {hhigh : idx < (aig.mkGateCached input).aig.decls.size} :
-    (aig.mkGateCached input).aig.decls[idx] matches .gate _ _ := by
-  simp only [mkGateCached, mkGateCached.go]
-  grind
-
-attribute [simp, grind! .] mkGateCached_decl_eq
-attribute [simp, grind! .] mkGateCached_le_size
+    ∃ (lhs rhs : Fanin), (aig.mkGateCached input).aig.decls[idx] = .gate lhs rhs := by
+  dsimp only [mkGateCached]
+  split <;> apply mkGateCached.go_matches_gate <;> trivial
 
 /--
 - `AIG.mkAndCached` only potentially appends gates, not atoms/constants
 -/
-@[simp, grind! .]
 theorem mkAndCached_matches_gate (idx : Nat) (aig : AIG α) (input : aig.BinaryInput)
     {hlow : idx ≥ aig.decls.size} {hhigh : idx < (aig.mkAndCached input).aig.decls.size} :
-    (aig.mkAndCached input).aig.decls[idx] matches .gate _ _ := by
-  simp_all [mkAndCached]
-
-attribute [simp, grind! .] mkAndCached_decl_eq
-attribute [simp, grind! .] mkAndCached_le_size
+    ∃ (lhs rhs : Fanin), (aig.mkAndCached input).aig.decls[idx] = .gate lhs rhs := by
+  simp_all only [mkAndCached, mkGateCached_matches_gate]
 
 end Valaig.Aig
