Valaig/Aiger/Basic.lean
@@ -1,0 +1,36 @@
+import Valaig.Aig.Basic
+
+namespace Valaig
+
+/--
+An extension of the sequential Aig to Aiger outputs
+-/
+structure Aiger extends Aig where
+  bads : Aig.Outputs
+
+  -- TODO: Other properties, invariants for them
+
+instance : Coe Aiger Aig where
+  coe := (·.toAig)
+
+namespace Aiger
+
+@[inline]
+def ofAig (aig : Aig) : Aiger :=
+  {
+    toAig := aig,
+    bads := #[]
+  }
+
+@[inline]
+def empty : Aiger :=
+  ofAig .empty
+
+@[inline, simp]
+abbrev numBads(aig : Aiger) : Nat := aig.bads.size
+
+@[inline]
+def addBad (aig : Aiger) (lit : Lit) (symbol : String := "") (_h : lit.validIn aig := by grind) : Aiger :=
+  { aig with bads := aig.bads.push { lit, symbol } }
+
+end Valaig.Aiger
