Valaig/Aiger/Lemmas.lean
@@ -1,0 +1,12 @@
+import Valaig.Aiger.Basic
+
+namespace Valaig.Aiger
+
+variable {aig : Aiger} {var : Var}
+
+@[grind .]
+theorem validIn_ofAig {aig : Aig} (h : var.validIn aig) :
+    var.validIn (ofAig aig) := by
+  simp_all only [ofAig]
+
+end Valaig.Aiger
